deps/poulet4/lib/P4automata/NtupleProofs.v
@@ -1,0 +1,124 @@
+Require Import Coq.Lists.List.
+Require Import Coq.NArith.BinNat.
+Require Import Poulet4.FinType.
+Require Import Poulet4.TypeNeq.
+Require Import Poulet4.P4automata.Ntuple.
+
+Definition next_tuple (n: nat) (t: n_tuple bool n) : n_tuple bool n.
+  revert t.
+  induction n; simpl; intros t; destruct t.
+  - exact tt.
+  - destruct b eqn:?.
+    + exact (IHn n0, false).
+    + exact (n0, true).
+Defined.
+
+Fixpoint enum_tuples' {n: nat} k (t: n_tuple bool n) :=
+  match k with
+  | 0 => nil
+  | S k => t :: enum_tuples' k (next_tuple n t)
+  end.
+
+Definition enum_tuples (n: nat) : list (n_tuple bool n) :=
+  enum_tuples' (Nat.pow 2 n) (n_tuple_repeat n false).
+
+Lemma length_enum_tuples':
+  forall {n} k (t: n_tuple bool n),
+    length (enum_tuples' k t) = k.
+Proof.
+  induction k; simpl; eauto.
+Qed.
+
+Lemma length_enum_tuples:
+  forall n,
+    length (enum_tuples n) = Nat.pow 2 n.
+Proof.
+  unfold enum_tuples.
+  eauto using length_enum_tuples'.
+Qed.
+
+Fixpoint code (n: nat) : n_tuple bool n -> nat :=
+  match n as n' return n_tuple bool n' -> nat with
+  | 0 => fun _ => 0
+  | S n =>
+    fun t =>
+    let '(t, b) := t in
+    match b with
+    | false => 2 * (code n t)
+    | true => S (2 * (code n t))
+    end
+  end.
+
+Lemma code_nth:
+  forall n (x: n_tuple bool n),
+    nth_error (enum_tuples n) (code n x) = Some x.
+Proof.
+  induction n.
+  - intros [].
+    reflexivity.
+  - unfold enum_tuples.
+    intros [x b].
+    cbn in *.
+    destruct b.
+Admitted.
+
+Global Program Instance BoolTupleFinite (n: nat): Finite (n_tuple bool n) :=
+  {| enum := enum_tuples n |}.
+Next Obligation.
+Admitted.
+Next Obligation.
+  eapply nth_error_In.
+  eapply code_nth.
+Qed.
+
+Lemma unit_type_neq:
+  forall T,
+    (unit:Type) = T ->
+    forall (x y: T),
+      x <> y ->
+      False.
+Proof.
+  intros T Ht.
+  rewrite <- Ht.
+  intros [] [].
+  congruence.
+Qed.
+
+Lemma n_tuple_diff_neq:
+  forall n m,
+    n <> m ->
+    n_tuple bool n <> n_tuple bool m.
+Proof.
+  intros.
+  eapply TypeNeq.card_neq.
+  cbn.
+  rewrite !length_enum_tuples.
+  intro Hpow.
+  eapply PeanoNat.Nat.pow_inj_r in Hpow; auto.
+Qed.
+
+Lemma n_tuple_succ_inj:
+  forall n m,
+    n_tuple bool (1 + n) = n_tuple bool (1 + m) ->
+    n_tuple bool n = n_tuple bool m.
+Proof.
+  intros n m.
+  destruct (PeanoNat.Nat.eq_dec n m).
+  - subst m.
+    eauto.
+  - intros.
+    exfalso.
+    eapply n_tuple_diff_neq; [|eassumption].
+    eauto.
+Qed.
+
+Lemma n_tuple_inj:
+  forall n m,
+    n_tuple bool n = n_tuple bool m ->
+    n = m.
+Proof.
+  intros.
+  destruct (PeanoNat.Nat.eq_dec n m); auto.
+  exfalso.
+  eapply n_tuple_diff_neq; eauto.
+Qed.
