deps/poulet4/lib/TypeNeq.v
@@ -1,0 +1,38 @@
+Require Import Coq.Lists.List.
+Require Import Coq.Arith.PeanoNat.
+Require Import Poulet4.FinType.
+
+Section TypeNeq.
+  Context (A B: Type).
+  Context `{Finite A}.
+  Context `{Finite B}.
+  Lemma card_eq_raw:
+    A = B ->
+    forall (xs: list A) (ys: list B),
+      (forall x, In x xs) ->
+      (forall y, In y ys) ->
+      NoDup xs ->
+      NoDup ys ->
+      length xs = length ys.
+  Proof.
+    intro eq.
+    subst B.
+    intros.
+    eapply Nat.le_antisymm;
+      eapply NoDup_incl_length;
+      unfold incl;
+      eauto.
+  Qed.
+
+  Lemma card_neq:
+    card A <> card B ->
+    A <> B.
+  Proof.
+    unfold "<>".
+    unfold card.
+    destruct H0, H2.
+    eauto using card_eq_raw.
+  Qed.
+
+End TypeNeq.
+
